correctness/RegexCorrectness/Backtracker/Basic.lean
@@ -1,0 +1,337 @@
+import Regex.Backtracker
+
+set_option autoImplicit false
+
+namespace Regex.Backtracker
+
+set_option linter.unusedVariables false in
+theorem captureNextAux.induct' (σ : Strategy) (nfa : NFA) (wf : nfa.WellFormed) (startIdx maxIdx : Nat)
+  (motive : BitMatrix nfa.nodes.size (maxIdx + 1 - startIdx) → List (StackEntry σ nfa startIdx maxIdx) → Prop)
+  (base : ∀ (visited : BitMatrix nfa.nodes.size (maxIdx + 1 - startIdx)), motive visited [])
+  (visited :
+    ∀ (visited : BitMatrix nfa.nodes.size (maxIdx + 1 - startIdx)) (update : σ.Update)
+      (state : Fin nfa.nodes.size) (it : BoundedIterator startIdx) (eq : it.maxIdx = maxIdx)
+      (stack' : List (StackEntry σ nfa startIdx maxIdx)),
+    visited.get state (it.index' eq) →
+    motive visited stack' →
+    motive visited (⟨update, state, it, eq⟩ :: stack'))
+  (done :
+    ∀ (visited : BitMatrix nfa.nodes.size (maxIdx + 1 - startIdx)) (update : σ.Update)
+      (state : Fin nfa.nodes.size) (it : BoundedIterator startIdx) (eq : it.maxIdx = maxIdx)
+      (stack' : List (StackEntry σ nfa startIdx maxIdx)),
+    ¬visited.get state (it.index' eq) →
+    nfa[state] = NFA.Node.done →
+    motive visited (⟨update, state, it, eq⟩ :: stack'))
+  (fail :
+    ∀ (visited : BitMatrix nfa.nodes.size (maxIdx + 1 - startIdx)) (update : σ.Update)
+      (state : Fin nfa.nodes.size) (it : BoundedIterator startIdx) (eq : it.maxIdx = maxIdx)
+      (stack' : List (StackEntry σ nfa startIdx maxIdx)),
+    ¬visited.get state (it.index' eq) →
+    nfa[state] = NFA.Node.fail →
+    motive visited (⟨update, state, it, eq⟩ :: stack'))
+  (epsilon :
+    ∀ (visited : BitMatrix nfa.nodes.size (maxIdx + 1 - startIdx)) (update : σ.Update)
+      (state : Fin nfa.nodes.size) (it : BoundedIterator startIdx) (eq : it.maxIdx = maxIdx)
+      (stack' : List (StackEntry σ nfa startIdx maxIdx)),
+    ¬visited.get state (it.index' eq) →
+    let visited' := visited.set state (it.index' eq);
+    ∀ (state' : Fin nfa.nodes.size),
+    nfa[state] = NFA.Node.epsilon state' →
+    motive visited' (⟨update, state', it, eq⟩ :: stack') →
+    motive visited (⟨update, state, it, eq⟩ :: stack'))
+  (split :
+    ∀ (visited : BitMatrix nfa.nodes.size (maxIdx + 1 - startIdx)) (update : σ.Update)
+      (state : Fin nfa.nodes.size) (it : BoundedIterator startIdx) (eq : it.maxIdx = maxIdx)
+      (stack' : List (StackEntry σ nfa startIdx maxIdx)),
+    ¬visited.get state (it.index' eq) →
+    let visited' := visited.set state (it.index' eq);
+    ∀ (state₁ state₂ : Fin nfa.nodes.size),
+    nfa[state] = NFA.Node.split state₁ state₂ →
+    motive visited' (⟨update, state₁, it, eq⟩ :: ⟨update, state₂, it, eq⟩ :: stack') →
+    motive visited (⟨update, state, it, eq⟩ :: stack'))
+  (save :
+    ∀ (visited : BitMatrix nfa.nodes.size (maxIdx + 1 - startIdx)) (update : σ.Update)
+      (state : Fin nfa.nodes.size) (it : BoundedIterator startIdx) (eq : it.maxIdx = maxIdx)
+      (stack' : List (StackEntry σ nfa startIdx maxIdx)),
+    ¬visited.get state (it.index' eq) →
+    let visited' := visited.set state (it.index' eq);
+    ∀ (offset : Nat) (state' : Fin nfa.nodes.size),
+    nfa[state] = NFA.Node.save offset state' →
+    let update' := σ.write update offset it.pos;
+    motive visited' (⟨update', state', it, eq⟩ :: stack') →
+    motive visited (⟨update, state, it, eq⟩ :: stack'))
+  (anchor_pos :
+    ∀ (visited : BitMatrix nfa.nodes.size (maxIdx + 1 - startIdx)) (update : σ.Update)
+      (state : Fin nfa.nodes.size) (it : BoundedIterator startIdx) (eq : it.maxIdx = maxIdx)
+      (stack' : List (StackEntry σ nfa startIdx maxIdx)),
+    ¬visited.get state (it.index' eq) →
+    let visited' := visited.set state (it.index' eq);
+    ∀ (a : Data.Anchor) (state' : Fin nfa.nodes.size),
+    nfa[state] = NFA.Node.anchor a state' →
+    Data.Anchor.test it.it a →
+    motive visited' (⟨update, state', it, eq⟩ :: stack') →
+    motive visited (⟨update, state, it, eq⟩ :: stack'))
+  (anchor_neg :
+    ∀ (visited : BitMatrix nfa.nodes.size (maxIdx + 1 - startIdx)) (update : σ.Update)
+      (state : Fin nfa.nodes.size) (it : BoundedIterator startIdx) (eq : it.maxIdx = maxIdx)
+      (stack' : List (StackEntry σ nfa startIdx maxIdx)),
+    ¬visited.get state (it.index' eq) →
+    let visited' := visited.set state (it.index' eq);
+    ∀ (a : Data.Anchor) (state' : Fin nfa.nodes.size),
+    nfa[state] = NFA.Node.anchor a state' →
+    ¬Data.Anchor.test it.it a →
+    motive visited' stack' →
+    motive visited (⟨update, state, it, eq⟩ :: stack'))
+  (char_pos :
+    ∀ (visited : BitMatrix nfa.nodes.size (maxIdx + 1 - startIdx)) (update : σ.Update)
+      (state : Fin nfa.nodes.size) (it : BoundedIterator startIdx) (eq : it.maxIdx = maxIdx)
+      (stack' : List (StackEntry σ nfa startIdx maxIdx)),
+    ¬visited.get state (it.index' eq) →
+    let visited' := visited.set state (it.index' eq);
+    ∀ (c : Char) (state' : Fin nfa.nodes.size),
+    nfa[state] = NFA.Node.char c state' →
+    (h : it.hasNext) →
+    it.curr h = c →
+    motive visited' (⟨update, state', it.next h, eq⟩ :: stack') →
+    motive visited (⟨update, state, it, eq⟩ :: stack'))
+  (char_neg :
+    ∀ (visited : BitMatrix nfa.nodes.size (maxIdx + 1 - startIdx)) (update : σ.Update)
+      (state : Fin nfa.nodes.size) (it : BoundedIterator startIdx) (eq : it.maxIdx = maxIdx)
+      (stack' : List (StackEntry σ nfa startIdx maxIdx)),
+    ¬visited.get state (it.index' eq) →
+    let visited' := visited.set state (it.index' eq);
+    ∀ (c : Char) (state' : Fin nfa.nodes.size),
+    nfa[state] = NFA.Node.char c state' →
+    (h : it.hasNext) →
+    ¬it.curr h = c →
+    motive visited' stack' →
+    motive visited (⟨update, state, it, eq⟩ :: stack'))
+  (char_end :
+    ∀ (visited : BitMatrix nfa.nodes.size (maxIdx + 1 - startIdx)) (update : σ.Update)
+      (state : Fin nfa.nodes.size) (it : BoundedIterator startIdx) (eq : it.maxIdx = maxIdx)
+      (stack' : List (StackEntry σ nfa startIdx maxIdx)),
+    ¬visited.get state (it.index' eq) →
+    let visited' := visited.set state (it.index' eq);
+    ∀ (c : Char) (state' : Fin nfa.nodes.size),
+    nfa[state] = NFA.Node.char c state' →
+    ¬it.hasNext →
+    motive visited' stack' →
+    motive visited (⟨update, state, it, eq⟩ :: stack'))
+  (sparse_pos :
+    ∀ (visited : BitMatrix nfa.nodes.size (maxIdx + 1 - startIdx)) (update : σ.Update)
+      (state : Fin nfa.nodes.size) (it : BoundedIterator startIdx) (eq : it.maxIdx = maxIdx)
+      (stack' : List (StackEntry σ nfa startIdx maxIdx)),
+    ¬visited.get state (it.index' eq) →
+    let visited' := visited.set state (it.index' eq);
+    ∀ (cs : Data.Classes) (state' : Fin nfa.nodes.size),
+    nfa[state] = NFA.Node.sparse cs state' →
+    (h : it.hasNext) →
+    it.curr h ∈ cs →
+    motive visited' (⟨update, state', it.next h, eq⟩ :: stack') →
+    motive visited (⟨update, state, it, eq⟩ :: stack'))
+  (sparse_neg :
+    ∀ (visited : BitMatrix nfa.nodes.size (maxIdx + 1 - startIdx)) (update : σ.Update)
+      (state : Fin nfa.nodes.size) (it : BoundedIterator startIdx) (eq : it.maxIdx = maxIdx)
+      (stack' : List (StackEntry σ nfa startIdx maxIdx)),
+    ¬visited.get state (it.index' eq) →
+    let visited' := visited.set state (it.index' eq);
+    ∀ (cs : Data.Classes) (state' : Fin nfa.nodes.size),
+    nfa[state] = NFA.Node.sparse cs state' →
+    (h : it.hasNext) →
+    ¬it.curr h ∈ cs →
+    motive visited' stack' →
+    motive visited (⟨update, state, it, eq⟩ :: stack'))
+  (sparse_end :
+    ∀ (visited : BitMatrix nfa.nodes.size (maxIdx + 1 - startIdx)) (update : σ.Update)
+      (state : Fin nfa.nodes.size) (it : BoundedIterator startIdx) (eq : it.maxIdx = maxIdx)
+      (stack' : List (StackEntry σ nfa startIdx maxIdx)),
+    ¬visited.get state (it.index' eq) →
+    let visited' := visited.set state (it.index' eq);
+    ∀ (cs : Data.Classes) (state' : Fin nfa.nodes.size),
+    nfa[state] = NFA.Node.sparse cs state' →
+    ¬it.hasNext →
+    motive visited' stack' →
+    motive visited (⟨update, state, it, eq⟩ :: stack'))
+  (matrix : BitMatrix nfa.nodes.size (maxIdx + 1 - startIdx)) (stack : List (StackEntry σ nfa startIdx maxIdx)) :
+  motive matrix stack :=
+  captureNextAux.induct σ nfa wf startIdx maxIdx motive base visited
+    (fun visited update state it eq stack' mem _ hn =>
+      done visited update state it eq stack' mem hn)
+    (fun visited update state it eq stack' mem _ hn =>
+      fail visited update state it eq stack' mem hn)
+    (fun visited update state it eq stack' mem _ state' hn isLt ih =>
+      epsilon visited update state it eq stack' mem ⟨state', isLt⟩ hn ih)
+    (fun visited update state it eq stack' mem _ state₁ state₂ hn isLt ih =>
+      split visited update state it eq stack' mem ⟨state₁, isLt.1⟩ ⟨state₂, isLt.2⟩ hn ih)
+    (fun visited update state it eq stack' mem _ offset state' hn isLt ih =>
+      save visited update state it eq stack' mem offset ⟨state', isLt⟩ hn ih)
+    (fun visited update state it eq stack' mem _ a state' hn isLt ih =>
+      anchor_pos visited update state it eq stack' mem a ⟨state', isLt⟩ hn ih)
+    (fun visited update state it eq stack' mem _ a state' hn isLt ih =>
+      anchor_neg visited update state it eq stack' mem a ⟨state', isLt⟩ hn ih)
+    (fun visited update state it eq stack' mem _ state' isLt h hn ih =>
+      char_pos visited update state it eq stack' mem (it.curr h) ⟨state', isLt⟩ hn h rfl ih)
+    (fun visited update state it eq stack' mem _ c state' hn isLt h ne ih =>
+      char_neg visited update state it eq stack' mem c ⟨state', isLt⟩ hn h ne ih)
+    (fun visited update state it eq stack' mem _ c state' hn isLt h ih =>
+      char_end visited update state it eq stack' mem c ⟨state', isLt⟩ hn h ih)
+    (fun visited update state it eq stack' mem _ cs state' hn isLt h ih =>
+      sparse_pos visited update state it eq stack' mem cs ⟨state', isLt⟩ hn h ih)
+    (fun visited update state it eq stack' mem _ cs state' hn isLt h ih =>
+      sparse_neg visited update state it eq stack' mem cs ⟨state', isLt⟩ hn h ih)
+    (fun visited update state it eq stack' mem _ cs state' hn isLt h ih =>
+      sparse_end visited update state it eq stack' mem cs ⟨state', isLt⟩ hn h ih)
+    matrix stack
+
+/-
+Simplification lemmas for `captureNextAux`.
+-/
+section
+
+variable {σ nfa wf startIdx maxIdx visited}
+
+@[simp]
+theorem captureNextAux_base :
+  captureNextAux σ nfa wf startIdx maxIdx visited [] = (.none, visited) := by
+  simp [captureNextAux]
+
+@[simp]
+theorem captureNextAux_visited {update state it eq stack'} (mem : visited.get state (it.index' eq)) :
+  captureNextAux σ nfa wf startIdx maxIdx visited (⟨update, state, it, eq⟩ :: stack') = captureNextAux σ nfa wf startIdx maxIdx visited stack' := by
+  conv =>
+    lhs
+    unfold captureNextAux
+    simp [mem]
+
+@[simp]
+theorem captureNextAux_done {update state it eq stack'} (mem : ¬visited.get state (it.index' eq)) (hn : nfa[state] = .done) :
+  captureNextAux σ nfa wf startIdx maxIdx visited (⟨update, state, it, eq⟩ :: stack') = (.some update, visited.set state (it.index' eq)) := by
+  simp at hn
+  conv =>
+    lhs
+    unfold captureNextAux
+    simp [mem]
+  split <;> simp_all
+
+@[simp]
+theorem captureNextAux_fail {update state it eq stack'} (mem : ¬visited.get state (it.index' eq)) (hn : nfa[state] = .fail) :
+  captureNextAux σ nfa wf startIdx maxIdx visited (⟨update, state, it, eq⟩ :: stack') = (.none, visited.set state (it.index' eq)) := by
+  conv =>
+    lhs
+    unfold captureNextAux
+    simp [mem]
+  split <;> simp_all
+
+@[simp]
+theorem captureNextAux_epsilon {update state it eq stack' state'} (mem : ¬visited.get state (it.index' eq)) (hn : nfa[state] = .epsilon state') :
+  captureNextAux σ nfa wf startIdx maxIdx visited (⟨update, state, it, eq⟩ :: stack') =
+  captureNextAux σ nfa wf startIdx maxIdx (visited.set state (it.index' eq)) (⟨update, state', it, eq⟩ :: stack') := by
+  conv =>
+    lhs
+    unfold captureNextAux
+    simp [mem]
+  split <;> simp_all
+
+@[simp]
+theorem captureNextAux_split {update state it eq stack' state₁ state₂} (mem : ¬visited.get state (it.index' eq)) (hn : nfa[state] = .split state₁ state₂) :
+  captureNextAux σ nfa wf startIdx maxIdx visited (⟨update, state, it, eq⟩ :: stack') =
+  captureNextAux σ nfa wf startIdx maxIdx (visited.set state (it.index' eq)) (⟨update, state₁, it, eq⟩ :: ⟨update, state₂, it, eq⟩ :: stack') := by
+  conv =>
+    lhs
+    unfold captureNextAux
+    simp [mem]
+  split <;> simp_all
+
+@[simp]
+theorem captureNextAux_save {update state it eq stack' offset state'} (mem : ¬visited.get state (it.index' eq)) (hn : nfa[state] = .save offset state') :
+  captureNextAux σ nfa wf startIdx maxIdx visited (⟨update, state, it, eq⟩ :: stack') =
+  captureNextAux σ nfa wf startIdx maxIdx (visited.set state (it.index' eq)) (⟨σ.write update offset it.pos, state', it, eq⟩ :: stack') := by
+  conv =>
+    lhs
+    unfold captureNextAux
+    simp [mem]
+  split <;> simp_all
+
+@[simp]
+theorem captureNextAux_anchor_pos {update state it eq stack' a state'} (mem : ¬visited.get state (it.index' eq)) (hn : nfa[state] = .anchor a state') (h : Data.Anchor.test it.it a) :
+  captureNextAux σ nfa wf startIdx maxIdx visited (⟨update, state, it, eq⟩ :: stack') =
+  captureNextAux σ nfa wf startIdx maxIdx (visited.set state (it.index' eq)) (⟨update, state', it, eq⟩ :: stack') := by
+  conv =>
+    lhs
+    unfold captureNextAux
+    simp [mem]
+  split <;> simp_all
+
+@[simp]
+theorem captureNextAux_anchor_neg {update state it eq stack' a state'} (mem : ¬visited.get state (it.index' eq)) (hn : nfa[state] = .anchor a state') (h : ¬Data.Anchor.test it.it a) :
+  captureNextAux σ nfa wf startIdx maxIdx visited (⟨update, state, it, eq⟩ :: stack') =
+  captureNextAux σ nfa wf startIdx maxIdx (visited.set state (it.index' eq)) stack' := by
+  conv =>
+    lhs
+    unfold captureNextAux
+    simp [mem]
+  split <;> simp_all
+
+@[simp]
+theorem captureNextAux_char_pos {update state it eq stack' c state'} (mem : ¬visited.get state (it.index' eq)) (hn : nfa[state] = .char c state') (h : it.hasNext) (hc : it.curr h = c) :
+  captureNextAux σ nfa wf startIdx maxIdx visited (⟨update, state, it, eq⟩ :: stack') =
+  captureNextAux σ nfa wf startIdx maxIdx (visited.set state (it.index' eq)) (⟨update, state', it.next h, eq⟩ :: stack') := by
+  conv =>
+    lhs
+    unfold captureNextAux
+    simp [mem]
+  split <;> simp_all
+
+@[simp]
+theorem captureNextAux_char_neg {update state it eq stack' c state'} (mem : ¬visited.get state (it.index' eq)) (hn : nfa[state] = .char c state') (h : it.hasNext) (hc : ¬it.curr h = c) :
+  captureNextAux σ nfa wf startIdx maxIdx visited (⟨update, state, it, eq⟩ :: stack') =
+  captureNextAux σ nfa wf startIdx maxIdx (visited.set state (it.index' eq)) stack' := by
+  conv =>
+    lhs
+    unfold captureNextAux
+    simp [mem]
+  split <;> simp_all
+
+@[simp]
+theorem captureNextAux_char_end {update state it eq stack' c state'} (mem : ¬visited.get state (it.index' eq)) (hn : nfa[state] = .char c state') (h : ¬it.hasNext) :
+  captureNextAux σ nfa wf startIdx maxIdx visited (⟨update, state, it, eq⟩ :: stack') =
+  captureNextAux σ nfa wf startIdx maxIdx (visited.set state (it.index' eq)) stack' := by
+  conv =>
+    lhs
+    unfold captureNextAux
+    simp [mem]
+  split <;> simp_all
+
+@[simp]
+theorem captureNextAux_sparse_pos {update state it eq stack' cs state'} (mem : ¬visited.get state (it.index' eq)) (hn : nfa[state] = .sparse cs state') (h : it.hasNext) (hc : it.curr h ∈ cs) :
+  captureNextAux σ nfa wf startIdx maxIdx visited (⟨update, state, it, eq⟩ :: stack') =
+  captureNextAux σ nfa wf startIdx maxIdx (visited.set state (it.index' eq)) (⟨update, state', it.next h, eq⟩ :: stack') := by
+  conv =>
+    lhs
+    unfold captureNextAux
+    simp [mem]
+  split <;> simp_all
+
+@[simp]
+theorem captureNextAux_sparse_neg {update state it eq stack' cs state'} (mem : ¬visited.get state (it.index' eq)) (hn : nfa[state] = .sparse cs state') (h : it.hasNext) (hc : ¬it.curr h ∈ cs) :
+  captureNextAux σ nfa wf startIdx maxIdx visited (⟨update, state, it, eq⟩ :: stack') =
+  captureNextAux σ nfa wf startIdx maxIdx (visited.set state (it.index' eq)) stack' := by
+  conv =>
+    lhs
+    unfold captureNextAux
+    simp [mem]
+  split <;> simp_all
+
+@[simp]
+theorem captureNextAux_sparse_end {update state it eq stack' cs state'} (mem : ¬visited.get state (it.index' eq)) (hn : nfa[state] = .sparse cs state') (h : ¬it.hasNext) :
+  captureNextAux σ nfa wf startIdx maxIdx visited (⟨update, state, it, eq⟩ :: stack') =
+  captureNextAux σ nfa wf startIdx maxIdx (visited.set state (it.index' eq)) stack' := by
+  conv =>
+    lhs
+    unfold captureNextAux
+    simp [mem]
+  split <;> simp_all
+
+end
+
+end Regex.Backtracker
