correctness/RegexCorrectness/Backtracker/Traversal.lean
@@ -1,0 +1,111 @@
+import RegexCorrectness.Backtracker.Basic
+
+set_option autoImplicit false
+
+namespace Regex.Backtracker.captureNextAux
+
+variable {σ nfa wf it startIdx maxIdx visited stack update visited'}
+
+theorem mem_of_mem_visited {s i} (hmem : visited.get s i) :
+  (captureNextAux σ nfa wf startIdx maxIdx visited stack).2.get s i := by
+  induction visited, stack using captureNextAux.induct' σ nfa wf startIdx maxIdx with
+  | base visited => simp [hmem]
+  | visited visited update state it eq stack' mem ih => simp [mem, ih hmem]
+  | done visited update state bit eq stack' mem hn => simp [mem, hn, BitMatrix.get_set, hmem]
+  | fail visited update state bit eq stack' mem hn => simp [mem, hn, BitMatrix.get_set, hmem]
+  | epsilon visited update state it eq stack' mem visited' state' hn ih =>
+    rw [captureNextAux_epsilon mem hn]
+    exact ih (by simp [visited', BitMatrix.get_set, hmem])
+  | split visited update state it eq stack' mem visited' state₁ state₂ hn ih =>
+    rw [captureNextAux_split mem hn]
+    exact ih (by simp [visited', BitMatrix.get_set, hmem])
+  | save visited update state it eq stack' mem visited' offset state' hn update' ih =>
+    rw [captureNextAux_save mem hn]
+    exact ih (by simp [visited', BitMatrix.get_set, hmem])
+  | anchor_pos visited update state it eq stack' mem visited' a state' hn ht ih =>
+    rw [captureNextAux_anchor_pos mem hn ht]
+    exact ih (by simp [visited', BitMatrix.get_set, hmem])
+  | anchor_neg visited update state it eq stack' mem visited' a state' hn ht ih =>
+    rw [captureNextAux_anchor_neg mem hn ht]
+    exact ih (by simp [visited', BitMatrix.get_set, hmem])
+  | char_pos visited update state it eq stack' mem visited' c state' hn hnext hc ih =>
+    rw [captureNextAux_char_pos mem hn hnext hc]
+    exact ih (by simp [visited', BitMatrix.get_set, hmem])
+  | char_neg visited update state it eq stack' mem visited' c state' hn hnext hc ih =>
+    rw [captureNextAux_char_neg mem hn hnext hc]
+    exact ih (by simp [visited', BitMatrix.get_set, hmem])
+  | char_end visited update state it eq stack' mem visited' c state' hn hnext ih =>
+    rw [captureNextAux_char_end mem hn hnext]
+    exact ih (by simp [visited', BitMatrix.get_set, hmem])
+  | sparse_pos visited update state it eq stack' mem visited' cs state' hn hnext hc ih =>
+    rw [captureNextAux_sparse_pos mem hn hnext hc]
+    exact ih (by simp [visited', BitMatrix.get_set, hmem])
+  | sparse_neg visited update state it eq stack' mem visited' cs state' hn hnext hc ih =>
+    rw [captureNextAux_sparse_neg mem hn hnext hc]
+    exact ih (by simp [visited', BitMatrix.get_set, hmem])
+  | sparse_end visited update state it eq stack' mem visited' cs state' hn hnext ih =>
+    rw [captureNextAux_sparse_end mem hn hnext]
+    exact ih (by simp [visited', BitMatrix.get_set, hmem])
+
+theorem mem_of_mem_top_stack {entry stack'} (hstack : entry :: stack' = stack) :
+  (captureNextAux σ nfa wf startIdx maxIdx visited stack).2.get entry.state (entry.it.index' entry.eq) := by
+  induction visited, stack using captureNextAux.induct' σ nfa wf startIdx maxIdx with
+  | base visited => simp at hstack
+  | visited visited update state it eq stack' mem ih =>
+    simp [mem]
+    simp at hstack
+    exact mem_of_mem_visited (by simp [hstack, mem])
+  | done visited update state bit eq stack' mem hn =>
+    simp [mem, hn]
+    simp at hstack
+    simp [hstack, BitMatrix.get_set]
+  | fail visited update state bit eq stack' mem hn =>
+    simp [mem, hn]
+    simp at hstack
+    simp [hstack, BitMatrix.get_set]
+  | epsilon visited update state it eq stack'' mem visited' state' hn ih =>
+    rw [captureNextAux_epsilon mem hn]
+    simp at hstack
+    exact mem_of_mem_visited (by simp [BitMatrix.get_set, hstack, mem])
+  | split visited update state it eq stack'' mem visited' state₁ state₂ hn ih =>
+    rw [captureNextAux_split mem hn]
+    simp at hstack
+    exact mem_of_mem_visited (by simp [BitMatrix.get_set, hstack, mem])
+  | save visited update state it eq stack' mem visited' offset state' hn update' ih =>
+    rw [captureNextAux_save mem hn]
+    simp at hstack
+    exact mem_of_mem_visited (by simp [BitMatrix.get_set, hstack, mem])
+  | anchor_pos visited update state it eq stack' mem visited' a state' hn ht ih =>
+    rw [captureNextAux_anchor_pos mem hn ht]
+    simp at hstack
+    exact mem_of_mem_visited (by simp [BitMatrix.get_set, hstack, mem])
+  | anchor_neg visited update state it eq stack' mem visited' a state' hn ht ih =>
+    rw [captureNextAux_anchor_neg mem hn ht]
+    simp at hstack
+    exact mem_of_mem_visited (by simp [BitMatrix.get_set, hstack, mem])
+  | char_pos visited update state it eq stack' mem visited' c state' hn hnext hc ih =>
+    rw [captureNextAux_char_pos mem hn hnext hc]
+    simp at hstack
+    exact mem_of_mem_visited (by simp [BitMatrix.get_set, hstack, mem])
+  | char_neg visited update state it eq stack' mem visited' c state' hn hnext hc ih =>
+    rw [captureNextAux_char_neg mem hn hnext hc]
+    simp at hstack
+    exact mem_of_mem_visited (by simp [BitMatrix.get_set, hstack, mem])
+  | char_end visited update state it eq stack' mem visited' c state' hn hnext ih =>
+    rw [captureNextAux_char_end mem hn hnext]
+    simp at hstack
+    exact mem_of_mem_visited (by simp [BitMatrix.get_set, hstack, mem])
+  | sparse_pos visited update state it eq stack' mem visited' cs state' hn hnext hc ih =>
+    rw [captureNextAux_sparse_pos mem hn hnext hc]
+    simp at hstack
+    exact mem_of_mem_visited (by simp [BitMatrix.get_set, hstack, mem])
+  | sparse_neg visited update state it eq stack' mem visited' cs state' hn hnext hc ih =>
+    rw [captureNextAux_sparse_neg mem hn hnext hc]
+    simp at hstack
+    exact mem_of_mem_visited (by simp [BitMatrix.get_set, hstack, mem])
+  | sparse_end visited update state it eq stack' mem visited' cs state' hn hnext ih =>
+    rw [captureNextAux_sparse_end mem hn hnext]
+    simp at hstack
+    exact mem_of_mem_visited (by simp [BitMatrix.get_set, hstack, mem])
+
+end Regex.Backtracker.captureNextAux
